AP/AP/Defense/Basic.lean
@@ -2,9 +2,13 @@ import AP.AP.Defense.Defs
 
 namespace AP.Defense
 
-theorem wf_def {dse : Defense} :
-dse.WF ↔ ∀ s [sys.WF s], dse.cnd s → ∀ (a : AStrat) [a.WF], ∀ (d : DStrat) [d.WF] n,
-(sys.simulate (Strat.f ⟨a, dse.st d⟩) s n).1.aPos ∉ dse.ps := ⟨λ ⟨h⟩ => h, λ h => ⟨h⟩⟩
+variable {dse : Defense}
+variable [wf : dse.WF]
+omit wf
+
+theorem wf_def : dse.WF ↔
+∀ s [sys.WF s], dse.cnd s → ∀ (a : AStrat) [a.WF], ∀ (d : DStrat) [d.WF] n,
+(sys.simulate (Strat.f ⟨a, dse.st d⟩) s n).1.aPos ∉ dse.ps := ⟨(·.1), (⟨·⟩)⟩
 
 instance : Inhabited Defense :=
   ⟨{cnd := λ _ => True, ps := ∅, f := λ _ => none}⟩
@@ -13,4 +17,4 @@ instance : Inhabited Defense :=
 theorem default_def : (default : Defense) =
 {cnd := λ _ => True, ps := ∅, f := λ _ => none} := rfl
 
-instance : WF default := ⟨by simp⟩
+@[simp] instance : WF default := ⟨by simp⟩
