AP/AP/Defense/Corner.lean
@@ -1,0 +1,71 @@
+import AP.AP.Defense.Edge
+
+namespace AP
+
+@[ext]
+structure Corner : Type where
+  dir : Dir
+  offset : PointZ
+deriving Inhabited, DecidableEq
+
+namespace Corner
+
+@[simp]
+def edge (dir : Dir) (offset : PointZ) : Edge where
+  dir := dir
+  offset := offset.coord dir
+
+def edge₁ (cor : Corner) : Edge :=
+  edge cor.dir cor.offset
+
+def edge₂ (cor : Corner) : Edge :=
+  edge cor.dir.rotRight cor.offset
+
+def points (cor : Corner) : Set PointZ :=
+  cor.edge₁.points ∪ cor.edge₂.points
+
+def memPoints (cor : Corner) (p : PointZ) : Bool :=
+  let ⟨x, y⟩ := p
+  let ⟨cx, cy⟩ := cor.offset
+  match cor.dir with
+  | .up => y ≤ cy ∨ cx ≤ x
+  | .right => cx ≤ x ∨ cy ≤ y
+  | .down => cy ≤ y ∨ x ≤ cx
+  | .left => x ≤ cx ∨ y ≤ cy
+
+theorem mem_points_iff_memPoints {cor : Corner} {p} :
+p ∈ cor.points ↔ cor.memPoints p := by
+  simp [points, edge₁, edge₂, memPoints, Edge.points]
+  cases cor.dir <;> simp [Edge.memPoints]
+
+instance {cor : Corner} {p} : Decidable # p ∈ cor.points :=
+  match h : cor.memPoints p with
+  | true => .isTrue # by simp [mem_points_iff_memPoints, h]
+  | false => .isFalse # by simp [mem_points_iff_memPoints, h]
+
+@[simp]
+theorem memPoints_eq {cor : Corner} {p} : cor.memPoints p = decide (p ∈ cor.points) := by
+  simp [mem_points_iff_memPoints]
+
+-- theorem points_inj {c₁ c₂ : Corner} (h : c₁.points = c₂.points) : c₁ = c₂ := by
+--   sorry
+
+-- @[simp]
+-- theorem points_eq_points_iff {e₁ e₂ : Corner} : e₁.points = e₂.points ↔ e₁ = e₂ :=
+--   ⟨points_inj, λ h => by rw [h]⟩
+
+def dist (cor : Corner) (p : PointZ) : ℤ :=
+  min (cor.edge₁.dist p) (cor.edge₂.dist p)
+
+def defenseCnd (cor : Corner) (s : State) : Prop :=
+  6 ≤ cor.dist s.aPos ∧ ∀ (p : PointZ), cor.dist p = 0 →
+  7 ≤ p.dist cor.offset → p ∈ s.taken
+
+def defenseFn (cor : Corner) (s : State) : Option PointZ :=
+  cor.edge₁.defense.f s <|> cor.edge₂.defense.f s
+
+def defense (cor : Corner) : Defense :=
+  { cnd := λ s => 6 ≤ cor.dist s.aPos
+  , ps := cor.points
+  , f := cor.defenseFn
+  }
